impl_language.thy
@@ -1,0 +1,177 @@
+theory impl_language
+  imports Main 
+    "~~/src/HOL/Library/Monad_Syntax"
+"~~/src/HOL/Library/State_Monad"
+  repliss_sem
+begin
+
+context begin
+
+(*
+datatype iostate =
+    WaitInput
+    | WaitOutput int
+    | Idle
+*)
+
+(* let's build an io monad as an example*)
+datatype 'a io = 
+    WaitInput (onInput: "int \<Rightarrow> 'a io") 
+  | WaitOutput int (onOutput: "'a io") 
+  | Done 'a
+
+definition io_write :: "int \<Rightarrow> unit io" where
+"io_write i = WaitOutput i (Done ()) "
+
+definition io_read :: "int io" where
+"io_read = WaitInput (\<lambda>i. (Done i))"
+
+function (domintros) bind :: "'a io \<Rightarrow> ('a \<Rightarrow> 'b io) \<Rightarrow> 'b io"  where
+"bind (WaitInput oi) f = (WaitInput (\<lambda>i. bind (oi i) f)) "
+| "bind (WaitOutput i n) f = (WaitOutput i (bind n f)) "
+| "bind (Done v) f = (f v)"
+
+  by (pat_completeness, auto)
+termination
+proof auto
+  fix io :: "'a io" and f :: "'a \<Rightarrow> 'b io"
+  show "bind_dom (io, f)"
+  proof (induct io)
+    case (WaitInput x)
+    then show ?case
+      by (simp add: bind.domintros(1)) 
+  next
+    case (WaitOutput x1a io)
+    then show ?case
+      using bind.domintros(2) by blast 
+  next
+    case (Done x)
+    then show ?case
+      by (simp add: bind.domintros(3))
+  qed
+qed
+
+adhoc_overloading Monad_Syntax.bind bind
+
+definition proc :: "int io" where
+ "proc \<equiv>  do {
+  x \<leftarrow> io_read;
+  y \<leftarrow> io_read;
+  io_write (x+y);
+  Done (x*y)
+}"
+
+datatype action = In int | Out int
+
+inductive step :: "'a io \<Rightarrow> action list \<Rightarrow> 'a \<Rightarrow> bool" where
+step_done: "step (Done x) [] x"
+| step_in: "step (f x) tr y \<Longrightarrow>  step (WaitInput f) (In x#tr) y"
+| step_out: "step n tr y \<Longrightarrow>  step (WaitOutput x n) (Out x#tr) y"
+
+lemma "step proc [In 3, In 4, Out 7] 12"
+  find_theorems name: "impl_language.bind"
+  by (auto simp add: proc_def  io_read_def io_write_def intro!: step_in step_out step_done)
+
+fun single_step:: "'a io \<Rightarrow> (bool \<times> 'a io) option" where
+"single_step (WaitInput f) = Some (True, f 0)"
+| "single_step (WaitOutput i n) = Some (False, n)"
+| "single_step (Done i) = None"
+
+lemma "single_step proc = Some (True, WaitInput (\<lambda>i. WaitOutput i (Done 0)))"
+  by (auto simp add: proc_def  io_read_def io_write_def bind.psimps bind.domintros)
+
+
+
+definition proc2 :: "int list io" where
+ "proc2 \<equiv>  do {
+  x \<leftarrow> io_read;
+  y \<leftarrow> io_read;
+  io_write (x+y);
+  Done [x,y]
+}"
+
+
+(* example *)
+
+
+(*type_synonym ('localState, 'any) procedureImpl = "'localState \<Rightarrow> ('localState, 'any) localAction"*)
+
+
+(* lets *)
+
+typ "('a,'b) localAction"
+
+
+
+
+(* symbolic values *)
+datatype sval = SVal nat 
+
+datatype sym_localAction =
+    SymLocalStep
+  | SymBeginAtomic
+  | SymEndAtomic
+  | SymNewId 
+  | SymDbOperation operation "sval list"
+  | SymReturn sval
+
+type_synonym ('a,'s) step = "'s \<Rightarrow> (sym_localAction \<times> 'a \<times> 's)"
+
+fun bind :: "('a,'s) step \<Rightarrow> ('a \<Rightarrow> ('b,'s) step) \<Rightarrow> ('b,'s) step"  where
+"bind s f = (\<lambda>x. let (a,r,s') = s x in f r s')"
+
+definition "s_newid" :: "('a, 's) step" where
+"s_newid \<equiv> "
+
+(* symbolic state *)
+datatype 'a sym_state = 
+  SymState 'a "nat" "sym_localAction list"
+
+
+fun bind :: "'a sym_state \<Rightarrow> ('a \<Rightarrow> 'b sym_state) \<Rightarrow> 'b sym_state"  where
+"bind (x i as) = "
+
+datatype cmd = 
+    Call "int"
+  | Seq "cmd" "cmd"
+  | Return int
+  | Skip
+
+datatype 'any lstate = LState (ls_val:"'any") (ls_cmd:"cmd")
+
+
+definition bind :: "'a lstate \<Rightarrow> ('a \<Rightarrow> 'b lstate) \<Rightarrow> 'b lstate"  where
+"bind s f \<equiv> let s' = f (ls_val s) in LState (ls_val s') (Seq (ls_cmd s) (ls_cmd s'))"
+
+adhoc_overloading Monad_Syntax.bind bind
+
+definition call :: "int \<Rightarrow> int lstate" where
+ "call c \<equiv> LState (2*c) (Call c)"
+
+definition "return x \<equiv> LState x Skip"
+
+definition "test1 \<equiv> bind (call 2) (return)"
+
+definition proc :: "int lstate" where
+ "proc \<equiv>  do {
+  x \<leftarrow> call 1;
+  y \<leftarrow> call (x+1);
+  return y
+}"
+
+lemma "proc = ???"
+  thm proc_def
+  apply (auto simp add: proc_def)
+  apply (auto simp add: bind_def Let_def call_def return_def)
+
+lemma "run test 0 = ???"
+  apply (auto simp add: test_def run_def op_a_def op_b_def bind_def return_def split: ) 
+  oops
+
+definition run :: "'any blub \<Rightarrow>  ('localState, 'any) procedureImpl"
+  where "run \<equiv> ???"
+
+end
+
+
+end
